Organizes STMonad Interface using a typeclass.

tests/monadic/stmonad/stmonad.cpp
@@ -1,1 +1,1 @@
-#include <stmonad.h>
+#include "stmonad.h"
