tests/monadic/stmonad/STMonadtest.v
@@ -11,6 +11,7 @@ From Stdlib Require Import
   Relation_Definitions
   Setoid
   Strings.String
+  Classes.EquivDec
 .
 
 From Crane Require Import Monads.ITree.
@@ -43,38 +44,34 @@ Import ListNotations.
 Import ProperNotations.
 Local Open Scope monad_scope.
 Local Open Scope string_scope.
-Import ST_IMPL.
 
 
+
+  
 
 Section ExampleTrees.
 
-  Context {S : Type}.
   Context {E : Type -> Type}.
-  Context `{IdxGenE -< E}.
+  Context {S : Type}.
+  (* Variable (ltu : T -> T -> Prop). *)
+  Context `{Ix_Correct nat Nat.le}.
+  Context {HST: STRefClass nat}.
+
+  Let V : nat -> Type := fun _ => nat. (* Nats only for this example. *)
+  Context {HSEv: STEvent nat S V -< E}. 
   Context `{exceptE Err -< E}.
+  Let E0 := (STEvent nat S V) +' E.
 
 
-  Definition V : Idx S -> Type := fun _ => nat.
-  Definition E0 := (STEvent S V) +' E.
-
-(* newSTRef :
- * forall {E : Type -> Type} {S : Type} (V : Idx S -> Type),
- * STEvent S V -< E -> forall I : Idx S, V I -> itree E (STRef S (V I)) *)
-  About readSTRef.
-(* readSTRef :
- * forall {E : Type -> Type} {S : Type} (V : Idx S -> Type),
- * STEvent S V -< E -> forall I : Idx S, STRef S (V I) -> itree E (V I) *)
-  (* TODO: tricky to state below! *)
   Definition newAndReadBoth : itree E0 (nat * nat) :=
-    r1 <- newSTRef V _ 5 ;;
-    r2 <- newSTRef V _ 6 ;;
-    x1 <- readSTRef V _ r1 ;;
-    x2 <- readSTRef V _ r2 ;;
-    Ret (x1, x2).
+      r1 <- newSTRef zero 5 ;;
+      r2 <- newSTRef (suc zero) 6 ;; (* TODO: autogenerate successive indices? *)
+      x1 <- readSTRef r1 ;;
+      x2 <- readSTRef r2 ;;
+      Ret (x1, x2).
 
   Definition tree_simp : itree E0 nat :=
-    v <- newSTRef 5;;
+    v <- newSTRef zero 5;;
     readSTRef v.
 
   (* NOTE: this failing definition is intentional.
@@ -85,22 +82,84 @@ Section ExampleTrees.
     readSTRef v.
 
   Definition tree_simp_another : itree E0 nat :=
-    v <- newSTRef 5;;
+    v <- newSTRef zero 5;;
     writeSTRef v 6;;
     val <- readSTRef v;;
     Ret val.
 
 
+   Definition swap' (v w : STRef S nat) : itree E0 unit :=
+    a <- @readSTRef E0 nat S  _ V  _ (STRefToIx _ _ v) v;;
+    b <- @readSTRef E0 nat S _ V _ (STRefToIx _ _ w) w;;
+    writeSTRef v b;;
+    writeSTRef w a.
+
   (* "swap" function from "Lazy Functional State Threads", by John Launchbury and Simon L Peyton Jones. *)
-  Definition swap (v w : STRef S nat) : itree E0 unit :=
+  (* TODO: would be good for indices here to be inferrable. *)
+  Fail Definition swap (v w : STRef S nat) : itree E0 unit :=
     a <- readSTRef v;;
     b <- readSTRef w;;
     writeSTRef v b;;
     writeSTRef w a.
 
+
+
+  (* TODO: Quicksort Example in haskell. *)
+
+(* import Control.Monad.ST
+ * import Data.Array.ST
+ * import Data.Foldable
+ * import Control.Monad
+ * 
+ * -- wiki-copied code starts here
+ * partition arr left right pivotIndex = do
+ *     pivotValue <- readArray arr pivotIndex
+ *     swap arr pivotIndex right
+ *     storeIndex <- foreachWith [left..right-1] left (\i storeIndex -> do
+ *         val <- readArray arr i
+ *         if (val <= pivotValue)
+ *             then do
+ *                  swap arr i storeIndex
+ *                  return (storeIndex + 1)
+ *             else do
+ *                  return storeIndex )
+ *     swap arr storeIndex right
+ *     return storeIndex
+ * 
+ * qsort arr left right = when (right > left) $ do
+ *     let pivotIndex = left + ((right-left) `div` 2)
+ *     newPivot <- partition arr left right pivotIndex
+ * 
+ *     qsort arr left (newPivot - 1)
+ *     qsort arr (newPivot + 1) right
+ * 
+ * -- wrapper to sort a list as an array
+ * sortList xs = runST $ do
+ *     let lastIndex = length xs - 1
+ *     arr <- newListArray (0,lastIndex) xs :: ST s (STUArray s Int Int)
+ *     qsort arr 0 lastIndex
+ *     newXs <- getElems arr
+ *     return newXs
+ * 
+ * -- test example
+ * main = print $ sortList [212498,127,5981,2749812,74879,126,4,51,2412]
+ * 
+ * -- helpers
+ * swap arr left right = do
+ *     leftVal <- readArray arr left
+ *     rightVal <- readArray arr right
+ *     writeArray arr left rightVal
+ *     writeArray arr right leftVal
+ * 
+ * -- foreachWith takes a list, and a value that can be modified by the function, and
+ * -- it returns the modified value after mapping the function over the list.  
+ * foreachWith xs v f = foldlM (flip f) v xs *)
+  
 End ExampleTrees.
 
 
-From Crane Require Import Mapping.NatIntStd.   
-Crane Extract Skip E0.
+
+(* Crane Extract Skip Ix. *)
+Require Import Crane.Mapping.NatIntStd.
 Crane Extraction "stmonad" newAndReadBoth tree_simp tree_simp_another.
+
